sha update
checkpoint

update

investigations/cava2/Sha256.v
@@ -23,33 +23,110 @@ Require Import Cava.Types.
 Require Import Cava.Expr.
 Require Import Cava.Primitives.
 
+Require Import Cava.Fifo.
+
 Import ListNotations.
-Import ExprNotations.
 Import PrimitiveNotations.
 
 Local Open Scope string_scope.
 Local Open Scope N.
 
 Section Var.
+  Import ExprNotations.
+
   Context {var : tvar}.
 
-  Definition sha_round := BitVec 6.
+  Definition sha_round := BitVec 7.
   Definition sha_word := BitVec 32.
   Definition sha_block := Vec sha_word 16.
   Definition sha_digest := Vec sha_word 8.
 
+  Definition padder_waiting := Constant (0: denote_type (BitVec 4)).
+  Definition padder_emit_bit := Constant (1: denote_type (BitVec 4)).
+  Definition padder_flushing := Constant (2: denote_type (BitVec 4)).
+  Definition padder_writing_length := Constant (3: denote_type (BitVec 4)).
+
   (* SHA-256 message padding *)
-  Definition sha256_padder : Circuit _ [Bit; BitVec 32; Bit; Bit] (sha_block ** Bit) := {{
-    fun data_valid data finish clear =>
-    (* TODO *)
-    `circuit_hole`
+  Definition sha256_padder : Circuit _ [Bit; BitVec 32; Bit; BitVec 4; Bit] (Bit ** sha_word ** Bit) :=
+    {{
+    fun data_valid data final final_byte_length back_pressure =>
+    let/delay '(done, out, out_valid, state, length; current_offset) :=
+      if !back_pressure
+      then (done, out, out_valid, state, length, current_offset)
+      else
+
+      let next_state :=
+        if final && state == `padder_waiting` then
+          if final_byte_length == `K 4`
+          then `padder_emit_bit`
+          else `padder_flushing`
+        else if state == `padder_emit_bit` then
+          `padder_flushing`
+        else if state == `padder_flushing` then
+          if current_offset == `K 61`
+          then `padder_writing_length`
+          else `padder_flushing`
+        else if state == `padder_writing_length` then
+          if current_offset == `K 63`
+          then `padder_waiting`
+          else `padder_writing_length`
+        else
+          state
+        in
+
+      let next_length :=
+        if state == `padder_waiting` && data_valid then length + `K 4`
+        else if state == `padder_waiting` && final then length + `resize` final_byte_length
+        else if state == `padder_writing_length` && current_offset == `K 62`
+          then `K 0`
+        else length
+        in
+
+      let next_out :=
+        if state == `padder_waiting` && final then
+          if final_byte_length == `K 0`
+          then `Constant (0x00000001: denote_type (BitVec 32))`
+          else if final_byte_length == `K 1`
+          then `slice 0 8` data ++ `Constant (0x000001: denote_type (BitVec 24))`
+          else if final_byte_length == `K 2`
+          then `slice 0 16` data ++ `Constant (0x0001: denote_type (BitVec 16))`
+          else if final_byte_length == `K 3`
+          then `slice 0 24` data ++ `Constant (0x01: denote_type (BitVec 8))`
+          else data
+        else if state == `padder_waiting` && data_valid then
+          data
+        else if state == `padder_emit_bit` then
+          `Constant (0x00000001: denote_type (BitVec 32))`
+        else if state == `padder_writing_length` then
+          if current_offset == `K 62`
+          then `reverse` (`slice 32 32` length)
+          else `reverse` (`slice 0 32` length)
+
+        else `K 0`
+      in
+
+      let step :=
+        (state == `padder_waiting` && (data_valid || final))
+        || (! (state == `padder_waiting`) ) in
+
+      let next_offset := if step then current_offset + `K 1` else current_offset in
+
+      ( state == `padder_writing_length` && next_state == `padder_waiting`
+      , next_out, step, next_state, next_length, next_offset)
+
+      initially
+        (false,(0,(false,(0,(0,0)))))
+        : denote_type (Bit ** sha_word ** Bit ** BitVec 4 ** BitVec 61 ** BitVec 16)
+        in
+
+    (out_valid, out, done)
   }}.
+
 
   (* SHA-256 initial digest *)
   Definition sha256_initial_digest : denote_type sha_digest :=
-    List.map (HexString.to_N)
-    [ "0x6a09e667" ; "0xbb67ae85" ; "0x3c6ef372" ; "0xa54ff53a"
-    ; "0x510e527f" ; "0x9b05688c" ; "0x1f83d9ab" ; "0x5be0cd19" ].
+    [ 0x6a09e667 ; 0xbb67ae85 ; 0x3c6ef372 ; 0xa54ff53a
+    ; 0x510e527f ; 0x9b05688c ; 0x1f83d9ab ; 0x5be0cd19 ]%list.
 
   (* SHA-256 round constants *)
   Definition sha256_round_constants : Circuit [] [sha_round] sha_word := {{
@@ -57,23 +134,22 @@ Section Var.
     let k :=
     `
     Constant (
-    List.map (HexString.to_N)
-    [ "0x428a2f98"; "0x71374491"; "0xb5c0fbcf"; "0xe9b5dba5"
-    ; "0x3956c25b"; "0x59f111f1"; "0x923f82a4"; "0xab1c5ed5"
-    ; "0xd807aa98"; "0x12835b01"; "0x243185be"; "0x550c7dc3"
-    ; "0x72be5d74"; "0x80deb1fe"; "0x9bdc06a7"; "0xc19bf174"
-    ; "0xe49b69c1"; "0xefbe4786"; "0x0fc19dc6"; "0x240ca1cc"
-    ; "0x2de92c6f"; "0x4a7484aa"; "0x5cb0a9dc"; "0x76f988da"
-    ; "0x983e5152"; "0xa831c66d"; "0xb00327c8"; "0xbf597fc7"
-    ; "0xc6e00bf3"; "0xd5a79147"; "0x06ca6351"; "0x14292967"
-    ; "0x27b70a85"; "0x2e1b2138"; "0x4d2c6dfc"; "0x53380d13"
-    ; "0x650a7354"; "0x766a0abb"; "0x81c2c92e"; "0x92722c85"
-    ; "0xa2bfe8a1"; "0xa81a664b"; "0xc24b8b70"; "0xc76c51a3"
-    ; "0xd192e819"; "0xd6990624"; "0xf40e3585"; "0x106aa070"
-    ; "0x19a4c116"; "0x1e376c08"; "0x2748774c"; "0x34b0bcb5"
-    ; "0x391c0cb3"; "0x4ed8aa4a"; "0x5b9cca4f"; "0x682e6ff3"
-    ; "0x748f82ee"; "0x78a5636f"; "0x84c87814"; "0x8cc70208"
-    ; "0x90befffa"; "0xa4506ceb"; "0xbef9a3f7"; "0xc67178f2" ] : denote_type (Vec sha_word 64)
+    [ 0x428a2f98; 0x71374491; 0xb5c0fbcf; 0xe9b5dba5
+    ; 0x3956c25b; 0x59f111f1; 0x923f82a4; 0xab1c5ed5
+    ; 0xd807aa98; 0x12835b01; 0x243185be; 0x550c7dc3
+    ; 0x72be5d74; 0x80deb1fe; 0x9bdc06a7; 0xc19bf174
+    ; 0xe49b69c1; 0xefbe4786; 0x0fc19dc6; 0x240ca1cc
+    ; 0x2de92c6f; 0x4a7484aa; 0x5cb0a9dc; 0x76f988da
+    ; 0x983e5152; 0xa831c66d; 0xb00327c8; 0xbf597fc7
+    ; 0xc6e00bf3; 0xd5a79147; 0x06ca6351; 0x14292967
+    ; 0x27b70a85; 0x2e1b2138; 0x4d2c6dfc; 0x53380d13
+    ; 0x650a7354; 0x766a0abb; 0x81c2c92e; 0x92722c85
+    ; 0xa2bfe8a1; 0xa81a664b; 0xc24b8b70; 0xc76c51a3
+    ; 0xd192e819; 0xd6990624; 0xf40e3585; 0x106aa070
+    ; 0x19a4c116; 0x1e376c08; 0x2748774c; 0x34b0bcb5
+    ; 0x391c0cb3; 0x4ed8aa4a; 0x5b9cca4f; 0x682e6ff3
+    ; 0x748f82ee; 0x78a5636f; 0x84c87814; 0x8cc70208
+    ; 0x90befffa; 0xa4506ceb; 0xbef9a3f7; 0xc67178f2 ]%list : denote_type (Vec sha_word 64)
     )
     ` in
     `index` k i
@@ -88,28 +164,26 @@ Section Var.
   }}%nat.
 
   (* SHA-256 compression function *)
-  Program
   Definition sha256_compress : Circuit []%circuit_type [sha_digest; sha_word; sha_word]%circuit_type sha_digest := {{
     fun current_digest k w =>
     let '( a', b', c', d', e', f', g'; h' ) := `vec_as_tuple (n:=7)` current_digest in
 
     let s1 := (e' >>> `6`) ^ (e' >>> `11`) ^ (e' >>> `25`) in
-    let ch := (e' & f') ^ (e' & g') in
+    let ch := (e' & f') ^ (~e' & g') in
     let temp1 := (h' + s1 + ch + k + w) in
     let s0 := (a' >>> `2`) ^ (a' >>> `13`) ^ (a' >>> `22`) in
     let maj := (a' & b') ^ (a' & c') ^ (b' & c') in
     let temp2 := s0 + maj in
 
-
     (temp1 + temp2) :> a' :> b' :> c' :> (d' + temp1) :> e' :> f' :> g' :> []
   }}%nat.
 
   (* SHA-256 core *)
-  Definition sha256_inner : Circuit _ [sha_block; Bit; sha_digest] (sha_digest ** Bit) :=
+  Definition sha256_inner : Circuit _ [Bit; sha_block; sha_digest] (sha_digest ** Bit) :=
     {{
-    fun block block_valid initial_hash =>
+    fun block_valid block initial_digest =>
 
-    let/delay '(current_digest, message_schedule, done; round) :=
+    let/delay '(stored_digest, current_digest, message_schedule, done; round) :=
 
       let inc_round := !done in
       let start := (* done && *) block_valid in
@@ -117,7 +191,7 @@ Section Var.
       let k_i := `sha256_round_constants` round in
       let '(w0,w1, _, _, _, _, _, _
            , _,w9, _, _, _, _,w14;_ ) := `vec_as_tuple (n:=15)` message_schedule in
-      let update_schedule := round >= `K 16` in
+      let update_schedule := round >= `K 15` in
       let w16 :=
         if update_schedule
         then `sha256_message_schedule_update` w0 w1 w9 w14
@@ -127,27 +201,89 @@ Section Var.
         then message_schedule <<+ w16
         else message_schedule in
 
-      let next_digest := `sha256_compress` current_digest k_i w0 in
+      let next_digest := `sha256_compress` current_digest k_i
+        (`index` message_schedule (
+          if round >= `K 16`
+          then `K 15`
+          else round)
+        ) in
 
+      let done := (round == `K 64`) || done in
       let round := if inc_round then round + `K 1` else round in
-      let done := (round == `K 63`) || done in
 
       if start
-      then (initial_hash, block, `Constant ((false, 0):denote_type (Bit**sha_round))`)
-      else (next_digest, w, done, round)
+      then (initial_digest, initial_digest, block, `Constant ((false, 0):denote_type (Bit**sha_round))`)
+      else if done then (stored_digest, current_digest, message_schedule, done, round)
+      else (stored_digest, next_digest, w, done, round)
 
-      initially ((sha256_initial_digest, (repeat 0 16, (false, 0)))
-        : denote_type (sha_digest ** Vec sha_word 16 ** Bit ** sha_round )) in
+      initially ((sha256_initial_digest, (sha256_initial_digest, (repeat 0 16, (false, 0))))
+      : denote_type (sha_digest ** sha_digest ** sha_block ** Bit ** sha_round )) in
 
-    (current_digest, done)
+    let updated_digest := `map2 {{fun a b => ( a + b ) }} ` stored_digest current_digest in
+    (updated_digest, done)
 
   }}.
 
+  (* SHA-256 core *)
+  (* TODO(FIXME): *)
+  Definition sha256 : Circuit _ [Bit; sha_word; Bit; BitVec 4] (Bit ** sha_digest ** Bit) :=
+    {{ fun data_valid data final final_mask =>
+       let '(padded_valid, padded_data; padder_done) := `sha256_padder` data_valid data final final_mask `False` in
+
+       let/delay '(block, digest, count; busy) :=
+
+         let accept_fifo := !busy in
+
+         let '(fifo_valid, fifo_data; fifo_full) := `fifo (fifo_size := 999)` padded_valid padded_data accept_fifo in
+
+         let new_data := fifo_valid && accept_fifo in
+
+         let '(next_block;next_count) :=
+           if new_data
+           then (block <<+ fifo_data, count + `K 1`)
+           else (block, count)
+         in
+
+         let block_valid := `False` in
+         let '(inner_digest; inner_done) := `sha256_inner` block_valid block `Constant sha256_initial_digest` in
+
+         let next_digest := if inner_done then inner_digest else digest in
+
+         (next_block, inner_digest, next_count, busy)
+         initially (repeat 0 16, (sha256_initial_digest, (0,false))): denote_type (sha_block ** sha_digest ** BitVec 4 ** Bit) in
+
+       (busy, digest, busy)
+    }}.
+
 End Var.
 
-(* Section SanityCheck. *)
-(*   Require Import Cava.Semantics. *)
-(*   Time Compute step sha256_message_schedule_update tt (0,(3,(6,(9,tt)))). *)
-(*   Open Scope list_scope. *)
-(*   Time Compute step sha256_compress tt ([1;2;3;4;5;7;8;9],(1,(2,tt))). *)
-(* End SanityCheck. *)
+Section SanityCheck.
+  Require Import Cava.Semantics.
+  Open Scope list_scope.
+
+  Definition sha256_test_block : denote_type sha_block :=
+    [ 0x61626380; 0x00000000; 0x00000000; 0x00000000
+    ; 0x00000000; 0x00000000; 0x00000000; 0x00000000
+    ; 0x00000000; 0x00000000; 0x00000000; 0x00000000
+    ; 0x00000000; 0x00000000; 0x00000000; 0x00000018
+    ].
+
+  Definition init :=
+    step sha256_inner default (true, (sha256_test_block, (sha256_initial_digest, tt))).
+
+  Definition pp {n} (v: denote_type (Vec (BitVec 32) n)) :=
+      List.map HexString.of_N v.
+
+  (* Inner state holds the correct values after 64 rounds. *)
+  Goal
+    fst (snd (snd (simulate' sha256_inner (repeat (false, ([], ([], tt))) 64) (fst init)))) =
+    [0x506E3058; 0xD39A2165; 0x04D24D6C; 0xB85E2CE9; 0x5EF50F24; 0xFB121210; 0x948D25B6; 0x961F4894].
+  Proof. vm_compute. reflexivity. Qed.
+
+  (* Output is the correct message digest *)
+  Goal
+    fst (last (fst (simulate' sha256_inner (repeat (false, ([], ([], tt))) 64) (fst init))) default) =
+    [0xBA7816BF; 0x8F01CFEA; 0x414140DE; 0x5DAE2223; 0xB00361A3; 0x96177A9C; 0xB410FF61; 0xF20015AD ].
+  Proof. vm_compute. reflexivity. Qed.
+
+End SanityCheck.
